theories/memory.v
@@ -3,7 +3,7 @@
 From Coq Require Import BinNat.
 From Wasm Require Import bytes common.
 From HB Require Import structures.
-From mathcomp Require Import ssrbool eqtype.
+From mathcomp Require Import ssreflect ssrbool eqtype.
 
 Set Implicit Arguments.
 Unset Strict Implicit.
@@ -56,7 +56,8 @@ Section Memory.
         i <> i' ->
         mem_update i' b mem = Some mem' ->
         mem_lookup i mem' = mem_lookup i mem;
-      
+
+      (* Technically derivable from the others *)
       mem_update_length :
       forall i b mem mem',
         mem_update i b mem = Some mem' ->
@@ -84,6 +85,94 @@ Section Memory.
         mem_length mem' = N.add (mem_length mem) n;
     }.
 
-Context `{Memory}.
+  Context `{Memory}.
+  
+  Lemma mem_lookup_some_length: forall m i,
+      mem_lookup i m <> None ->
+      N.lt i (mem_length m).
+  Proof.
+    move => m i Hlookup.
+    destruct (N.ltb i (mem_length m)) eqn:Hlt; first by lias.
+    exfalso.
+    move/N.ltb_spec0 in Hlt.
+    by apply mem_lookup_oob in Hlt.
+  Qed.
+  
+  Lemma mem_lookup_none_length: forall m i,
+      mem_lookup i m = None ->
+      N.ge i (mem_length m).
+  Proof.
+    move => m i Hlookup.
+    destruct (N.ltb i (mem_length m)) eqn:Hlt; move/N.ltb_spec0 in Hlt; last done.
+    by apply mem_lookup_ib in Hlt.
+  Qed.
+  
+  Lemma mem_length_boundary : forall m i,
+      mem_lookup (N.pred i) m <> None ->
+      mem_lookup i m = None ->
+      mem_length m = i.
+  Proof.
+    move => m i Hlookup1 Hlookup2.
+    apply mem_lookup_some_length in Hlookup1.
+    apply mem_lookup_none_length in Hlookup2.
+    apply N.le_succ_l in Hlookup1.
+    by lias.
+  Qed.
   
 End Memory.
+
+Section BlockUpdateMemory.
+  
+  Class BlockUpdateMemory := {
+      m: Memory;
+      mem_update_gen: N -> N -> (N -> byte) -> mem_t -> option mem_t;
+      
+      mem_update_gen_ib:
+      forall n len gen m,
+        N.le (N.add n len) (mem_length m) ->
+        mem_update_gen n len gen m <> None;
+      
+      mem_update_gen_oob:
+      forall n len gen m,
+        N.gt (N.add n len) (mem_length m) ->
+        mem_update_gen n len gen m = None;
+      
+      mem_update_gen_lookup:
+      forall n len gen m m' i,
+        mem_update_gen n len gen m = Some m' ->
+        N.lt i len ->
+        mem_lookup (N.add n i) m' = Some (gen i);
+                                         
+      mem_update_gen_lookup_lt:
+      forall n len gen m m' i,
+        mem_update_gen n len gen m = Some m' ->
+        N.lt i n ->
+        mem_lookup i m' = mem_lookup i m;
+
+      mem_update_gen_lookup_ge:
+      forall n len gen m m' i,
+        mem_update_gen n len gen m = Some m' ->
+        N.ge i (N.add n len) ->
+        mem_lookup i m' = mem_lookup i m;
+    }.
+
+  #[global]
+    Instance memory_from_bum `{bum: BlockUpdateMemory} : Memory := m.
+  
+  Hint Resolve memory_from_bum : typeclass_instances.
+
+  Lemma mem_update_gen_length `{BlockUpdateMemory}: forall n len gen m m',
+      mem_update_gen n len gen m = Some m' ->
+      mem_length m = mem_length m'.
+  Proof.
+    move => n len gen m m' Hupdate.
+    apply mem_length_boundary.
+    - destruct (N.ltb (N.pred (mem_length m')) (N.add n len)) eqn:Hlt; move/N.ltb_spec0 in Hlt.
+      + destruct (N.ltb (N.pred (mem_length m')) n) eqn:Hlt2; move/N.ltb_spec0 in Hlt2.
+        { eapply mem_update_gen_lookup_lt in Hlt2; eauto.
+          admit.
+        }
+        
+  Admitted.
+  
+End BlockUpdateMemory.
